plf-current/Equiv.v
@@ -1532,7 +1532,7 @@ Close Scope imp_scope.
 
 Example havoc_example1 : empty_st =[ (HAVOC X)%imp ]=> (X !-> 0).
 Proof.
-  apply E_Havoc.Qed.
+  apply E_Havoc. Qed.
 
 Example havoc_example2 :
   empty_st =[ (SKIP;; HAVOC Z)%imp ]=> (Z !-> 42).
