vc/Verif_append.v
@@ -1,0 +1,378 @@
+(** * Verif_append: List segments, magic wand *)
+
+(** THIS CHAPTER IS JUST A STUB RIGHT NOW. *)
+
+(** This chapter should show how to prove the correctness
+ of adding up a list, two different ways:
+ - with list-segments
+ - with magic wand
+
+ Then it should show proofs of the [append] function,
+ two different ways:
+ - with list-segments
+ - with magic wand
+*)
+
+
+(* ================================================================= *)
+(** ** Here is a little C program, [reverse.c] *)
+
+(** 
+
+#include <stddef.h>
+
+struct list {int head; struct list *tail;};
+
+unsigned sumlist (struct list *p) {
+  unsigned s = 0;
+  struct list *t = p;
+  unsigned h;
+  while (t) {
+     h = t->head;
+     t = t->tail;
+     s = s + h;
+  }
+  return s;
+}
+
+struct list *append (struct list *x, struct list *y) {
+  struct list *t, *u;
+  if (x==NULL)
+    return y;
+  else {
+    t = x;
+    u = t->tail;
+    while (u!=NULL) {
+      t = u;
+      u = t->tail;
+    }
+    t->tail = y;
+    return x;
+  }
+}
+*)
+
+Require Import VST.floyd.proofauto.
+Require Import append.
+Instance CompSpecs : compspecs. make_compspecs prog. Defined.
+Definition Vprog : varspecs. mk_varspecs prog. Defined.
+
+(* ================================================================= *)
+(** ** Inductive definition of linked lists *)
+
+Definition t_list := Tstruct _list noattr.
+
+Fixpoint listrep (sigma: list val) (p: val) : mpred :=
+ match sigma with
+ | h::hs => 
+    EX y:val, 
+      data_at Tsh t_list (h,y) p  *  listrep hs y
+ | nil => 
+    !! (p = nullval) && emp
+ end.
+
+Arguments listrep sigma p : simpl never.
+
+(* ================================================================= *)
+(** ** Hint databases for spatial operators *)
+
+(** This is the same proof as in [Verif_reverse] *)
+Lemma listrep_local_facts:
+  forall sigma p,
+   listrep sigma p |--
+   !! (is_pointer_or_null p /\ (p=nullval <-> sigma=nil)).
+Proof.
+intros.
+revert p; induction sigma; intros p.
+-
+ unfold listrep.
+ entailer!.
+ split; auto.
+-
+ unfold listrep; fold listrep.
+ entailer.
+ entailer!.
+ split; intro.
+ * clear - H H2.
+   subst p.
+   eapply field_compatible_nullval; eauto.
+ * inversion H2.
+Qed.
+Hint Resolve listrep_local_facts : saturate_local.
+
+(** This is the same proof as in [Verif_reverse] *)
+Lemma listrep_valid_pointer:
+  forall sigma p,
+   listrep sigma p |-- valid_pointer p.
+Proof.
+ intros.
+ unfold listrep.
+ destruct sigma; simpl.
+* entailer!.
+* entailer!.
+  auto with valid_pointer.
+Qed.
+Hint Resolve listrep_valid_pointer : valid_pointer.
+
+(* ================================================================= *)
+(** ** Specification of the [sumlist] and [append] functions. *)
+Definition sum_int : list int -> int := fold_right Int.add Int.zero.
+
+Definition sumlist_spec : ident * funspec :=
+ DECLARE _sumlist
+  WITH sigma : list int, p: val
+  PRE  [ _p OF (tptr t_list) ]
+     PROP ()
+     LOCAL (temp _p p)
+     SEP (listrep (map Vint sigma) p)
+  POST [ (tptr t_list) ]
+     PROP () 
+     LOCAL (temp ret_temp (Vint (sum_int sigma)))
+     SEP (listrep(map Vint sigma) p).
+
+Definition append_spec :=
+ DECLARE _append
+  WITH sh : share, x: val, y: val, s1: list val, s2: list val
+  PRE [ _x OF (tptr t_list) , _y OF (tptr t_list)]
+     PROP(writable_share sh)
+     LOCAL (temp _x x; temp _y y)
+     SEP (listrep s1 x; listrep s2 y)
+  POST [ tptr t_list ]
+    EX r: val,
+     PROP()
+     LOCAL(temp ret_temp r)
+     SEP (listrep (s1++s2) r).
+
+Definition Gprog : funspecs :=
+         ltac:(with_library prog [ sumlist_spec; append_spec ]).
+
+(** In separation-logic assertions, how should one specify integer values?
+    Normally, one should use the mathematical integers, Coq's [Z] type.
+    Then, inject [Z] into the 32-bit machine integers using Int.repr,
+    then from those into CompCert values by Vint.  That is,
+    [Vint (Int.repr z)], where [z:Z] is a mathematical integer.
+
+    If [z] is too big to fit in a 32-bit integer, [Int.repr] will take
+    the low-order 32 bits (i.e., modulo 2^32).  To make sure that doesn't
+    happen (if you didn't intend it), usually you maintain the assertion
+    [Int.min_signed <= z <= Int.max_signed].  
+
+    In this program, we are adding up a list of integers.  If we wanted
+    to prove that every partial sum is in range, we'd need a complicated
+    precondition.  Instead, we'll prove something simpler:  that the
+    sum mod 2^32 is right.   
+
+    In the C language, signed integer arithmetic is not allowed to
+    overflow (you get undefined behavior), so we must write this program
+    to use unsigned ints.  For that, we want to reason about
+    32-bit machine integers directly, not about the mathematical integers.
+    Therefore we'll use values of type [int], that is [Int.int], the
+    type of 32-bit machine integers.  That's why, in [sumlist_spec],
+    we use [sigma: list int] in our specification, instead of a list of [Z].
+
+    Compare with the proof of [pop_and_add] in [Verif_triang],
+    where we _do_ prove that each partial sum doesn't overflow, and
+    we can use signed integer arithmetic. *)
+
+(* ================================================================= *)
+(** ** Proof of the [sumlist] function *)
+
+(** First, we prove a useful auxiliary lemma about [sum_int] *)
+
+Lemma sum_int_app:
+  forall a b, sum_int (a++b) = Int.add (sum_int a) (sum_int b).
+Proof.
+intros.
+induction a; simpl. rewrite Int.add_zero_l; auto.
+rewrite IHa. rewrite Int.add_assoc. auto.
+Qed.
+
+(** TODO: This proof needs cleanup, and lots more explanation.  **)
+Lemma body_sumlist: semax_body Vprog Gprog f_sumlist sumlist_spec.
+Proof.
+(** Here is the standard way to start a function-body proof:  
+    First, [start-function], then [forward]. **)
+start_function.
+forward.  (* s = 0; *)
+forward.  (* t = p; *)
+forward_while
+    (EX sigma2: list int, EX t: val,
+     PROP ()
+     LOCAL (temp _t t;
+            temp _s (Vint (Int.sub (sum_int sigma) (sum_int sigma2))))
+     SEP (listrep (map Vint sigma2) t;
+          listrep (map Vint sigma2) t -* listrep (map Vint sigma) p)).
+- (* Prove that current precondition implies loop invariant *)
+Exists sigma p.
+entailer!.
+apply wand_sepcon_adjoint. cancel.
+- (* Prove that loop invariant implies typechecking condition *)
+entailer!.
+- (* Prove that loop body preserves invariant *)
+assert_PROP (sigma2 <> nil). {
+  unfold listrep at 1. 
+  entailer!. 
+  assert (t=nullval) by intuition. 
+  subst; contradiction.
+}
+destruct sigma2 as [ | i r]; try contradiction.
+clear H.
+simpl map.
+unfold listrep at 1; fold listrep.
+Intros y.
+forward.
+forward.
+forward.
+Exists (r,y).
+entailer!.
+f_equal.
+rewrite <- Int.sub_add_l.
+rewrite (Int.add_commut i).
+rewrite Int.sub_shifted. auto.
+apply -> wand_sepcon_adjoint.
+assert (data_at Tsh t_list (Vint i, y) t * listrep (map Vint r) y 
+         |-- listrep (Vint i :: map Vint r) t).
+unfold listrep at 2; fold listrep. 
+Exists y; cancel.
+sep_apply H2; clear H2.
+apply modus_ponens_wand.
+-
+subst.
+forward.
+assert (map Vint sigma2 = nil) by intuition.
+destruct sigma2; inv H0.
+eapply derives_trans. apply modus_ponens_wand.
+entailer!.
+Qed.
+
+(* ================================================================= *)
+(** ** Proof of the [append] function *)
+
+(** TODO: This proof needs cleanup, and lots more explanation.  **)
+Definition lseg (s: list val) (x y : val) := 
+  ALL s': list val, listrep s' y -* listrep (s ++ s') x.
+
+Lemma lseg_nullval: forall s t, lseg s t nullval = listrep s t.
+Proof.  
+unfold lseg; intros.
+apply pred_ext.
+apply allp_left with (@nil val).
+unfold listrep at 1.
+rewrite prop_true_andp by auto.
+rewrite emp_wand.
+rewrite <- app_nil_end.
+auto.
+apply allp_right; intro s'.
+apply wand_sepcon_adjoint.
+unfold listrep at 2.
+destruct s'; simpl.
+rewrite <- app_nil_end. entailer!.
+Intros y.
+entailer!.
+destruct H0; contradiction H0.
+Qed.
+
+Lemma lseg_listrep: forall s t x y ,
+      lseg s x y * listrep t y |-- listrep (s++t) x.
+Proof.
+intros.
+unfold lseg.
+allp_left t.
+rewrite sepcon_comm.
+apply modus_ponens_wand.
+Qed.
+
+Lemma lseg_app:
+   forall s t x y z,
+      lseg s x y * lseg t y z |-- lseg (s++t) x z.
+Proof.
+  intros.
+ apply allp_right; intro u.
+ apply -> wand_sepcon_adjoint.
+ sep_apply (lseg_listrep t u y z).
+ sep_apply (lseg_listrep s (t++u) x y).
+ rewrite app_ass.
+ auto.
+Qed.
+  
+Lemma body_append: semax_body Vprog Gprog f_append append_spec.
+Proof.
+start_function.
+forward_if.
+{ (* then-clause *)
+ subst.
+ forward.
+ rewrite (proj1 H) by auto.
+ unfold listrep at 1. simpl app. Exists y. entailer!.
+}
+(* else-clause *)
+assert_PROP (s1 <> nil). {
+   unfold listrep at 1. 
+   entailer!.  intuition.
+  }
+destruct s1 as [ | h r]; try congruence. clear H H0.
+unfold listrep at 1; fold listrep.
+Intros u.
+forward.
+forward.
+forward_while 
+   (EX u:val, EX t:val, EX s': list val, 
+    EX i: val, EX r': list val,
+    PROP (s' ++ [i] ++ r' = [h] ++ r)
+    LOCAL (temp _u u; temp _t t; temp _x x; temp _y y)
+    SEP (lseg s' x t; lseg [i] t u; listrep r' u; listrep s2 y)).
+* (* Prove that the precondition implies the loop invariant *)
+ Exists u x (@nil val) h r. 
+ entailer. (* Cannot use entailer! here. *)
+ apply sepcon_derives; auto.
+ apply derives_trans with (emp * (lseg [h] x u * listrep r u)).
+ cancel.
+ unfold lseg. apply allp_right; intro s'. apply wand_sepcon_adjoint.
+ simpl.
+ unfold listrep at 2; fold listrep. Exists u; cancel.
+ rewrite sepcon_assoc. apply sepcon_derives; auto.
+ unfold lseg. apply allp_right; intro s'. apply wand_sepcon_adjoint.
+ simpl. cancel.
+* (* Prove that the loop test can evaluate *)
+ entailer!.
+* (* Prove the function body preserves the invariant *)
+ forward.
+ assert_PROP (r' <> nil) by (entailer!; intuition).
+ destruct r' as [ | j r']; try congruence. clear H0.
+ unfold listrep at 1; fold listrep.
+ Intros z.
+ forward.
+ Exists (z,u0,s'++[i],j,r').
+ entailer!.
+ rewrite app_ass; auto.
+ sep_apply (lseg_app s' [i] x t u0).
+ cancel.
+ unfold lseg. apply allp_right; intro. simpl.
+ apply wand_sepcon_adjoint.
+ unfold listrep at 2; fold listrep.
+ Exists z. cancel.
+ * (* After the loop *)
+subst u0.
+assert_PROP (r'=nil) by (entailer!; intuition).
+subst r'.
+rewrite lseg_nullval.
+rewrite <- app_nil_end in H.
+rename s' into s.
+unfold listrep at 1 2.
+Intros p. subst p.
+forward.
+forward.
+Exists x.
+entailer!.
+change (h :: r ++ s2) with (([h]++r)++s2).
+rewrite <- H.
+rewrite app_ass.
+clear.
+assert (data_at Tsh t_list (i, y) t * listrep s2 y |--
+           listrep (i::s2) t).
+ unfold listrep at 2; fold listrep; Exists y; cancel.            sep_apply H; clear H.                                           
+simpl.
+unfold lseg. allp_left (i::s2). 
+sep_apply (modus_ponens_wand (listrep (i::s2) t) (listrep (s++i::s2) x)).
+auto.
+Qed.
